WIP on NetworkTypes

fstar/new/NetworkTypes.fst
@@ -4,16 +4,20 @@ open Lib.IntTypes
 open Parser
 open Crypto
 
-noeq type kdf_label = {
+type hpke_public_key_nt = blbytes ({min=1; max=(pow2 16)-1})
+
+val ps_hpke_public_key: parser_serializer hpke_public_key_nt
+let ps_hpke_public_key = ps_bytes _
+
+noeq type kdf_label_nt = {
   length: uint16;
   label: blbytes ({min=7; max=255});
   context: blbytes ({min=0; max=(pow2 32)-1});
 }
 
-val ps_kdf_label: parser_serializer kdf_label
+val ps_kdf_label: parser_serializer kdf_label_nt
 let ps_kdf_label =
-  isomorphism
-    kdf_label
+  isomorphism kdf_label_nt
     (
       _ <-- ps_u16;
       _ <-- ps_bytes _;
@@ -22,15 +26,14 @@ let ps_kdf_label =
     (fun (|length, (|label, context|)|) -> {length=length; label=label; context=context;})
     (fun x -> (|x.length, (|x.label, x.context|)|))
 
-noeq type hpke_ciphertext = {
+noeq type hpke_ciphertext_nt = {
   kem_output: blbytes ({min=0; max=(pow2 16)-1});
   ciphertext: blbytes ({min=0; max=(pow2 16)-1});
 }
 
-val ps_hpke_ciphertext: parser_serializer hpke_ciphertext
+val ps_hpke_ciphertext: parser_serializer hpke_ciphertext_nt
 let ps_hpke_ciphertext =
-  isomorphism
-    hpke_ciphertext
+  isomorphism hpke_ciphertext_nt
     (
       _ <-- ps_bytes _;
       ps_bytes _
@@ -39,53 +42,221 @@ let ps_hpke_ciphertext =
     (fun x -> (|x.kem_output, x.ciphertext|))
 
 
-noeq type update_path_node (cs:ciphersuite) = {
-  public_key: hpke_public_key cs;
-  encrypted_path_secret: blseq hpke_ciphertext ps_hpke_ciphertext ({min=0; max=(pow2 32)-1});
+noeq type update_path_node_nt = {
+  public_key: hpke_public_key_nt;
+  encrypted_path_secret: blseq hpke_ciphertext_nt ps_hpke_ciphertext ({min=0; max=(pow2 32)-1});
 }
 
-val ps_update_path_node: cs:ciphersuite -> parser_serializer (update_path_node cs)
-let ps_update_path_node cs =
-  assume (1 <= hpke_public_key_length cs); //TODO
-  isomorphism
-    (update_path_node cs)
+val ps_update_path_node: parser_serializer update_path_node_nt
+let ps_update_path_node =
+  isomorphism update_path_node_nt
     (
-      _ <-- ps_lbytes (hpke_public_key_length cs);
+      _ <-- ps_hpke_public_key;
       ps_seq _ ps_hpke_ciphertext
     )
     (fun (|public_key, encrypted_path_secret|) -> {public_key=public_key; encrypted_path_secret=encrypted_path_secret;})
     (fun x -> (|x.public_key, x.encrypted_path_secret|))
 
-noeq type key_package (cs:ciphersuite) = {
+type protocol_version_nt =
+  | PV_reserved: protocol_version_nt
+  | PV_mls10: protocol_version_nt
+  | PV_unknown: n:nat{2 <= n /\ n <= 255} -> protocol_version_nt
+
+val ps_protocol_version: parser_serializer protocol_version_nt
+let ps_protocol_version =
+  isomorphism protocol_version_nt
+    ps_u8
+    (fun n ->
+      match v n with
+      | 0 -> PV_reserved
+      | 1 -> PV_mls10
+      | vn -> PV_unknown vn
+    )
+    (fun x ->
+      match x with
+      | PV_reserved -> u8 0
+      | PV_mls10 -> u8 1
+      | PV_unknown n -> u8 n
+    )
+
+type cipher_suite_nt =
+  | CS_reserved: cipher_suite_nt
+  | CS_mls10_128_dhkemx25519_aes128gcm_sha256_ed25519: cipher_suite_nt
+  | CS_mls10_128_dhkemp256_aes128gcm_sha256_p256: cipher_suite_nt
+  | CS_mls10_128_dhkemx25519_chacha20poly1305_sha256_ed25519: cipher_suite_nt
+  | CS_mls10_256_dhkemx448_aes256gcm_sha512_ed448: cipher_suite_nt
+  | CS_mls10_256_dhkemp521_aes256gcm_sha512_p521: cipher_suite_nt
+  | CS_mls10_256_dhkemx448_chacha20poly1305_sha512_ed448: cipher_suite_nt
+  | CS_unknown: n:nat{7 <= n /\ n < 0xff00} -> cipher_suite_nt
+  | CS_reserved_private_use: n:nat{0xff00 <= n /\ n <= 0xffff} -> cipher_suite_nt
+
+val ps_cipher_suite: parser_serializer cipher_suite_nt
+let ps_cipher_suite =
+  isomorphism cipher_suite_nt
+    ps_u16
+    (fun n ->
+      match v n with
+      | 0 -> CS_reserved
+      | 1 -> CS_mls10_128_dhkemx25519_aes128gcm_sha256_ed25519
+      | 2 -> CS_mls10_128_dhkemp256_aes128gcm_sha256_p256
+      | 3 -> CS_mls10_128_dhkemx25519_chacha20poly1305_sha256_ed25519
+      | 4 -> CS_mls10_256_dhkemx448_aes256gcm_sha512_ed448
+      | 5 -> CS_mls10_256_dhkemp521_aes256gcm_sha512_p521
+      | 6 -> CS_mls10_256_dhkemx448_chacha20poly1305_sha512_ed448
+      | vn ->
+        if vn < 0xff00 then CS_unknown vn
+        else CS_reserved_private_use vn
+    )
+    (fun x ->
+      match x with
+      | CS_reserved -> u16 0
+      | CS_mls10_128_dhkemx25519_aes128gcm_sha256_ed25519 -> u16 1
+      | CS_mls10_128_dhkemp256_aes128gcm_sha256_p256 -> u16 2
+      | CS_mls10_128_dhkemx25519_chacha20poly1305_sha256_ed25519 -> u16 3
+      | CS_mls10_256_dhkemx448_aes256gcm_sha512_ed448 -> u16 4
+      | CS_mls10_256_dhkemp521_aes256gcm_sha512_p521 -> u16 5
+      | CS_mls10_256_dhkemx448_chacha20poly1305_sha512_ed448 -> u16 6
+      | CS_unknown n -> u16 n
+      | CS_reserved_private_use n -> u16 n
+    )
+
+//TODO: these are signature algorithms supported in MLS ciphersuites, it is not complete
+//(see <https://tools.ietf.org/html/rfc8446#appendix-B.3.1.3>)
+type signature_scheme_nt =
+  | SA_ecdsa_secp256r1_sha256: signature_scheme_nt
+  | SA_ecdsa_secp521r1_sha512: signature_scheme_nt
+  | SA_ed25519: signature_scheme_nt
+  | SA_ed448: signature_scheme_nt
+  | SA_unknown: n:nat{n <> 0x0403 /\ n <> 0x0603 /\ n <> 0x0807 /\ n <> 0x0808 /\ n <= 0xffff} -> signature_scheme_nt
+
+val ps_signature_scheme: parser_serializer signature_scheme_nt
+let ps_signature_scheme =
+  isomorphism signature_scheme_nt
+    ps_u16
+    (fun n ->
+      match v n with
+      | 0x0403 -> SA_ecdsa_secp256r1_sha256
+      | 0x0603 -> SA_ecdsa_secp521r1_sha512
+      | 0x0807 -> SA_ed25519
+      | 0x0808 -> SA_ed448
+      | vn -> SA_unknown vn
+    )
+    (fun x ->
+      match x with
+      | SA_ecdsa_secp256r1_sha256 -> u16 0x0403
+      | SA_ecdsa_secp521r1_sha512 -> u16 0x0603
+      | SA_ed25519 -> u16 0x0807
+      | SA_ed448 -> u16 0x0808
+      | SA_unknown n -> u16 n
+    )
+
+type credential_type_nt =
+  | CT_reserved: credential_type_nt
+  | CT_basic: credential_type_nt
+  | CT_x509: credential_type_nt
+  | CT_unknown: n:nat{3 <= n /\ n < 0xff00} -> credential_type_nt
+  | CT_reserved_private_use: n:nat{0xff00 <= n /\ n <= 0xffff} -> credential_type_nt
+
+val ps_credential_type: parser_serializer credential_type_nt
+let ps_credential_type =
+  isomorphism credential_type_nt
+    ps_u16
+    (fun n ->
+      match v n with
+      | 0x0000 -> CT_reserved
+      | 0x0001 -> CT_basic
+      | 0x0002 -> CT_x509
+      | vn ->
+        if vn < 0xff00 then CT_unknown vn
+        else CT_reserved_private_use vn
+    )
+    (fun x ->
+      match x with
+      | CT_reserved -> u16 0x0000
+      | CT_basic -> u16 0x0001
+      | CT_x509 -> u16 0x0002
+      | CT_unknown n -> u16 n
+      | CT_reserved_private_use n -> u16 n
+    )
+
+noeq type basic_credential_nt = {
+  identity: blbytes ({min=0; max=(pow2 16)-1});
+  signature_scheme: signature_scheme_nt;
+  signature_key: blbytes ({min=0; max=(pow2 16)-1});
+}
+
+val ps_basic_credential: parser_serializer basic_credential_nt
+let ps_basic_credential =
+  isomorphism basic_credential_nt
+    (
+      _ <-- ps_bytes _;
+      _ <-- ps_signature_scheme;
+      ps_bytes _
+    )
+    (fun (|identity, (|signature_scheme, signature_key|)|) -> ({identity=identity; signature_scheme=signature_scheme; signature_key=signature_key;}))
+    (fun x -> (|x.identity, (|x.signature_scheme, x.signature_key|)|))
+
+type certificate_nt = blbytes ({min=0; max=(pow2 16)-1})
+
+val ps_certificate: parser_serializer certificate_nt
+let ps_certificate =
+  isomorphism certificate_nt
+    (ps_bytes _)
+    (fun x -> x)
+    (fun x -> x)
+
+noeq type credential_nt =
+  | C_basic: basic_credential_nt -> credential_nt
+  | C_x509: blseq certificate_nt ps_certificate ({min=1; max=(pow2 32)-1}) -> credential_nt
+  | C_other: c:credential_type_nt{~(CT_basic? c \/ CT_x509? c)} -> credential_nt
+
+//val ps_credential: parser_serializer credential_nt
+//let ps_credential =
+//  isomorphism credential_nt
+//    (
+//      credential_type <-- ps_credential_type;
+//      ((
+//      match credential_type with
+//      | CT_basic -> ps_basic_credential
+//      | CT_x509 -> ps_seq _ ps_certificate
+//      | _ -> admit()
+//      ) <: (match credential_type with |CT_basic -> parser_serializer basic_credential_nt |CT_x509 -> parser_serializer (blseq certificate_nt ps_certificate ({min=1; max=(pow2 32)-1})) |_ -> admit()))
+//    )
+//  (fun _ -> admit())
+//  //(fun (|credential_type, credential|) ->
+//  //  match credential_type with
+//  //  | CT_basic -> C_basic credential
+//  //  | CT_x509 -> C_x509 credential
+//  //  | _ -> admit()
+//  //)
+//  (fun x -> admit())
+
+noeq type key_package_nt = {
   //TODO
-  public_key: hpke_public_key cs;
+  public_key: hpke_public_key_nt;
   //TODO
 }
 
-val ps_key_package: cs:ciphersuite -> parser_serializer (key_package cs)
-let ps_key_package cs =
-  assume (1 <= hpke_public_key_length cs); //TODO
-  isomorphism
-    (key_package cs)
+val ps_key_package: parser_serializer key_package_nt
+let ps_key_package =
+  isomorphism key_package_nt
     (
-      ps_lbytes (hpke_public_key_length cs)
+      ps_hpke_public_key
     )
     (fun public_key -> {public_key=public_key})
     (fun x -> x.public_key)
 
-//TODO: this type will be converted to a `path` for TreeSync / TreeKEM. Should we parse a `path` directly and hide this internal record?
-noeq type update_path (cs:ciphersuite) = {
-  leaf_key_package: key_package cs;
-  nodes: blseq (update_path_node cs) (ps_update_path_node cs) ({min=0; max=(pow2 32)-1});
+noeq type update_path_nt = {
+  leaf_key_package: key_package_nt;
+  nodes: blseq update_path_node_nt ps_update_path_node ({min=0; max=(pow2 32)-1});
 }
 
-val ps_update_path: cs:ciphersuite -> parser_serializer (update_path cs)
-let ps_update_path cs =
-  isomorphism
-    (update_path cs)
+val ps_update_path: parser_serializer update_path_nt
+let ps_update_path =
+  isomorphism update_path_nt
     (
-      _ <-- ps_key_package cs;
-      ps_seq _ (ps_update_path_node cs)
+      _ <-- ps_key_package;
+      ps_seq _ ps_update_path_node
     )
     (fun (|leaf_key_package, nodes|) -> {leaf_key_package=leaf_key_package; nodes=nodes})
     (fun x -> (|x.leaf_key_package, x.nodes|))
